fairneris/examples/no_drop_dup.v
@@ -480,22 +480,17 @@ Definition initial_state shA shB :=
        state_ms := ∅; (* NB: Needs to be filled *) |}).
 
 Lemma no_drop_dup_continued_simulation shA shB :
-  ∃ (mtr : mtrace simple_fair_model),
-    trfirst mtr = model_draft.Start ∧
-    continued_simulation
-      valid_state_evolution_fairness
-      (trace_singleton $ initial_state shA shB)
-      (trace_singleton (trfirst mtr)).
+  continued_simulation
+    valid_state_evolution_fairness
+    (trace_singleton $ initial_state shA shB)
+    (trace_singleton init_state).
 Proof.
-  eexists (tr_singl model_draft.Start).
-  split; [done|].
   assert (anerisPreG (fair_model_to_model simple_fair_model)
                      (anerisΣ (fair_model_to_model simple_fair_model))) as HPreG.
   { apply _. }
   eapply (strong_simulation_adequacy_multiple _ _ _ _ _ {[saA;saB]});
     [simpl; lia| |set_solver|set_solver| |set_solver|set_solver|..| |]=> /=.
   { intros ℓ ζ Hmatch Henabled. rewrite /role_enabled_model in Henabled. simpl.
-    
     assert (ℓ = A_role ∨ ℓ = B_role) as [Heq|Heq] by set_solver; simplify_eq.
     - assert (ζ = ("0.0.0.0", 0%nat)) as ->.
       { rewrite /labels_match /locale_simple_label in Hmatch.
@@ -529,13 +524,8 @@ Proof.
   admit.
 Admitted.
 
-Theorem choose_nat_terminates shA shB extr :
-  trfirst extr = initial_state shA shB →
-  extrace_fairly_terminating extr.
+Theorem choose_nat_terminates shA shB :
+  fairly_terminating (initial_state shA shB).
 Proof.
-  intros Hexfirst.
-  destruct (no_drop_dup_continued_simulation shA shB) as (mtr & Hmtr & Hsim).
-  eapply continued_simulation_fair_termination_preserved; [|by rewrite Hexfirst].
-  rewrite /initial_reachable.
-  destruct mtr; simpl in *; rewrite Hmtr; done.
+  apply continued_simulation_fair_termination, no_drop_dup_continued_simulation.
 Qed.
